start of proof for cache based

compiler/lucky13_split_div64_log.ec
@@ -323,3 +323,59 @@ module M = {
   }
 }.
 
+equiv l1 : M.constant_time_lt_jasmin ~ M.constant_time_lt_jasmin :
+={M.leakages}
+==> ={M.leakages}.
+proof.
+proc; inline *; sim.
+qed.
+
+equiv l4 : M.rotate_offset_div ~ M.rotate_offset_div:
+={M.leakages, md_size, scan_start} /\
+(0 <= (to_uint (mac_start - scan_start)) < 2^8){1} /\ 
+(0 <= (to_uint (mac_start - scan_start)) < 2^8){2} /\
+(16 <= to_uint md_size <= 64){1}
+==> ={M.leakages}.
+proof.
+admitted.
+
+(* md_size : mac tag size --> public *)
+(* orig_len : length of record : header + data + mac tag + padding --> public *)
+(* out : mac tag is stored in out --> public *)
+(* rec : whole message including header, message, tag, padding --> public *)
+
+op wf_rec mem (rec:W64.t) (orig_len md_size : W32.t) = 
+ let mac_end = loadW32 mem (to_uint (rec + W64.of_int 4)) in
+ to_uint orig_len + 255 < W32.modulus /\
+ to_uint md_size <= to_uint mac_end /\ 
+ 1 <= to_uint orig_len - to_uint mac_end <= 256.
+
+lemma wf_rec_cond_md_size_mac_end mem rec orig_len md_size : 
+  16 <= W32.to_uint md_size <= 64 =>
+  wf_rec mem rec orig_len md_size =>
+  let mac_end = loadW32 mem (to_uint (rec + W64.of_int 4)) in
+  if (md_size + W32.of_int 256 \ult orig_len) then 
+     0 <= to_uint (mac_end - md_size - (orig_len - (md_size + W32.of_int 256))) < 256
+  else 0 <= to_uint (mac_end - md_size - W32.zero) < 256.
+proof.
+  rewrite /wf_rec /=.
+  pose mac_end := loadW32 _ _; move: mac_end => mac_end hmd [h1 [h2 h3]].
+  have -> : mac_end - md_size - (orig_len - (md_size + W32.of_int 256)) = 
+            mac_end - orig_len +  W32.of_int 256 by ring.
+  case: (md_size + (of_int 256)%W32 \ult orig_len); rewrite W32.ultE; last first.
+  rewrite W32.WRingA.subr0 W32.to_uintB 1:W32.uleE 1:// W32.to_uintD_small /= /#. 
+  have -> h : mac_end - orig_len + W32.of_int 256 = mac_end + W32.of_int 256 - orig_len by ring.
+  rewrite W32.to_uintB 1:W32.uleE; 1: by rewrite W32.to_uintD_small /= /#.
+  rewrite W32.to_uintD_small /= /#.
+qed.
+
+equiv l_final : M.ssl3_cbc_copy_mac_jasmin_cache ~ M.ssl3_cbc_copy_mac_jasmin_cache :
+={M.leakages, md_size, orig_len, out, rec} /\
+(loadW64 Glob.mem (to_uint (rec + (of_int 16)%W64))){1} = 
+(loadW64 Glob.mem (to_uint (rec + (of_int 16)%W64))){2} /\
+16 <= to_uint md_size{2} <= 64 /\
+(wf_rec Glob.mem rec orig_len md_size){1} /\ 
+(wf_rec Glob.mem rec orig_len md_size){2}  
+==> ={M.leakages}.
+proof.
+
